Naming

Semantics/Imp/Aexp.lean
@@ -1,21 +1,21 @@
 import Semantics.Imp.Lang
 
 namespace Aexp
-namespace Natural
+namespace BigStep
 
-private inductive big_step: Aexp × State -> Int -> Prop
-  | val: big_step (val n, _) n
-  | var: big_step (var v, s) (s v)
-  | add (ha: big_step (a, s) x) (ha': big_step (a', s) y):
-    big_step (a + a', s) (x + y)
-  | sub (ha: big_step (a, s) x) (ha': big_step (a', s) y):
-    big_step (a - a', s) (x - y)
-  | mul (ha: big_step (a, s) x) (ha': big_step (a', s) y):
-    big_step (a * a', s) (x * y)
+private inductive BigStep: Aexp × State -> Int -> Prop
+  | val: BigStep (val n, _) n
+  | var: BigStep (var v, s) (s v)
+  | add (ha: BigStep (a, s) x) (ha': BigStep (a', s) y):
+    BigStep (a + a', s) (x + y)
+  | sub (ha: BigStep (a, s) x) (ha': BigStep (a', s) y):
+    BigStep (a - a', s) (x - y)
+  | mul (ha: BigStep (a, s) x) (ha': BigStep (a', s) y):
+    BigStep (a * a', s) (x * y)
 
-infix:10 " ==> " => big_step
+infix:10 " ==> " => BigStep
 
-private instance big_step.equiv: Setoid Aexp where
+private instance BigStep.equiv: Setoid Aexp where
   r a a' := ∀{s n}, ((a, s) ==> n) = ((a', s) ==> n)
   iseqv := {
     refl := fun _ => rfl
@@ -24,11 +24,11 @@ private instance big_step.equiv: Setoid Aexp where
   }
 
 private example: ((var "x" + 5) + (9 - 7), s0) ==> 7 :=
-  big_step.add
-    (big_step.add big_step.var big_step.val)
-    (big_step.sub big_step.val big_step.val)
+  BigStep.add
+    (BigStep.add BigStep.var BigStep.val)
+    (BigStep.sub BigStep.val BigStep.val)
 
-end Natural
+end BigStep
 
 def reduce (a: Aexp) (s: State): Int :=
   match a with
@@ -54,43 +54,43 @@ section Equivalence
 
 -- relational definition is equal to recursive
 private theorem reduce.from_natural
-  (hbig_step: conf ==> n): conf.1 conf.2 = n :=
-  by induction hbig_step with
+  (hBigStep: conf ==> n): conf.1 conf.2 = n :=
+  by induction hBigStep with
   | add _ _ iha iha' => exact iha ▸ iha' ▸ rfl
   | sub _ _ iha iha' => exact iha ▸ iha' ▸ rfl
   | mul _ _ iha iha' => exact iha ▸ iha' ▸ rfl
   | _ => rfl
 
-private theorem Natural.from_reduce
+private theorem BigStep.from_reduce
   (hred: a s = n): (a, s) ==> n :=
   by induction a generalizing n with
-  | val a => exact hred ▸ big_step.val
-  | var a => exact hred ▸ big_step.var
+  | val a => exact hred ▸ BigStep.val
+  | var a => exact hred ▸ BigStep.var
   | add a a' iha iha' =>
-    exact hred ▸ big_step.add (iha rfl) (iha' rfl)
+    exact hred ▸ BigStep.add (iha rfl) (iha' rfl)
   | sub a a' iha iha' =>
-    exact hred ▸ big_step.sub (iha rfl) (iha' rfl)
+    exact hred ▸ BigStep.sub (iha rfl) (iha' rfl)
   | mul a a' iha iha' =>
-    exact hred ▸ big_step.mul (iha rfl) (iha' rfl)
+    exact hred ▸ BigStep.mul (iha rfl) (iha' rfl)
 
-private theorem big_step_eq_reduce:
+private theorem BigStep_eq_reduce:
   ((a, s) ==> n) = (a s = n) :=
-  propext (Iff.intro reduce.from_natural Natural.from_reduce)
+  propext (Iff.intro reduce.from_natural BigStep.from_reduce)
 
-private theorem big_step_eq_reduce':
+private theorem BigStep_eq_reduce':
   (a, s) ==> a s :=
-  Natural.from_reduce rfl
+  BigStep.from_reduce rfl
 
-private theorem big_step_eq_eq_reduce_eq:
-  Natural.big_step.equiv.r a a' <-> reduce.equiv.r a a' := by
+private theorem BigStep_eq_eq_reduce_eq:
+  BigStep.BigStep.equiv.r a a' <-> reduce.equiv.r a a' := by
   simp only [Setoid.r, eq_iff_iff]
   constructor
   . intro h s
     specialize @h s (a' s)
-    rw [big_step_eq_reduce, big_step_eq_reduce, eq_self, iff_true] at h
+    rw [BigStep_eq_reduce, BigStep_eq_reduce, eq_self, iff_true] at h
     exact h
   . intro h s _
-    rw [big_step_eq_reduce, big_step_eq_reduce]
+    rw [BigStep_eq_reduce, BigStep_eq_reduce]
     specialize @h s
     rw [h]
 
