Semantics/Imp/SmallStep.lean
@@ -2,31 +2,32 @@ import Semantics.Imp.Bexp
 import Semantics.ReflTransRel
 
 namespace Com
-namespace Structural
 
-inductive small_step: Com × State -> Com × State -> Prop where
+inductive SmallStep: Com × State -> Com × State -> Prop where
   | ass:
-    small_step (ass v a, s) (skip, s[v <- a s])
+    SmallStep (ass v a, s) (skip, s[v <- a s])
 
   | skipcat:
-    small_step (skip++c, s) (c, s)
+    SmallStep (skip++c, s) (c, s)
 
-  | cat (hstep: small_step (c, s) (c', s')):
-    small_step (c++c'', s) (c'++c'', s')
+  | cat (hstep: SmallStep (c, s) (c', s')):
+    SmallStep (c++c'', s) (c'++c'', s')
 
   | ifelse:
-    small_step (if b then c else c' end, s) (bif b s then c else c', s)
+    SmallStep (if b then c else c' end, s) (bif b s then c else c', s)
 
   | whileloop:
-    small_step (while b loop c end, s)
+    SmallStep (while b loop c end, s)
           (bif b s then c++while b loop c end else skip, s)
 
-infixl:10 " ~> " => small_step
+infixl:10 " ~> " => SmallStep
+
+namespace SmallStep
 
 private example:
   ([|x := 0; while x <= 2 loop x := x + 1 end|], s0) ~>
       ([|skip; while x <= 2 loop x := x + 1 end|], s0["x" <- 0]) :=
-  small_step.cat small_step.ass
+  cat ass
 
 theorem cat_eq:
   ((c++c'', s) ~> conf)
@@ -34,13 +35,13 @@ theorem cat_eq:
       ∨ (c = skip ∧ conf = (c'', s))) :=
   propext {
     mp := fun hmp => match hmp with
-      | small_step.skipcat => Or.inr (And.intro rfl rfl)
-      | small_step.cat h =>
+      | skipcat => Or.inr (And.intro rfl rfl)
+      | cat h =>
         Or.inl (Exists.intro _ (Exists.intro _ (And.intro h rfl))),
     mpr := fun hmpr => match hmpr with
       | Or.inl (Exists.intro _c' (Exists.intro _s' (And.intro hl hr))) =>
-        hr ▸ small_step.cat hl
-      | Or.inr (And.intro hl hr) => hl ▸ hr ▸ small_step.skipcat
+        hr ▸ cat hl
+      | Or.inr (And.intro hl hr) => hl ▸ hr ▸ skipcat
   }
 
 theorem cond_eq:
@@ -48,14 +49,14 @@ theorem cond_eq:
     = (b s ∧ conf = (c, s) ∨ b s = false ∧ conf = (c', s)) :=
   propext {
     mp := fun hmp => match hb: b s with
-      | false => match hmp with | small_step.ifelse => Or.inr (And.intro rfl (hb ▸ rfl))
-      | true => match hmp with | small_step.ifelse => Or.inl (And.intro rfl (hb ▸ rfl)),
+      | false => match hmp with | ifelse => Or.inr (And.intro rfl (hb ▸ rfl))
+      | true => match hmp with | ifelse => Or.inl (And.intro rfl (hb ▸ rfl)),
     mpr := fun hmpr =>
       let hss: conf = (bif b s then c else c', s) :=
         match hb: b s with
         | true => match hb ▸ hmpr with | Or.inl (And.intro _ hr) => hr
         | false => match hb ▸ hmpr with | Or.inr (And.intro _ hr) => hr
-      hss ▸ small_step.ifelse
+      hss ▸ ifelse
   }
 
 theorem cond_false (hb: b s = false):
@@ -66,28 +67,28 @@ theorem cond_false (hb: b s = false):
     mpr := fun mp => cond_eq ▸ Or.inr (And.intro hb mp)
   }
 
-infixl:10 " ~>* " => RTL small_step
+infixl:10 " ~>* " => RTL SmallStep
 
 theorem star.demo':
   ([|x := 2; while 0 <= x loop x := x + 1 end|], s0) ~>*
       ([|while 0 <= x loop x := x + 1 end|], s0["x" <- 2]) :=
-  RTL.head (small_step.cat small_step.ass) (RTL.head small_step.skipcat RTL.refl)
+  RTL.head (cat ass) (RTL.head skipcat RTL.refl)
 
 theorem star.cat_skip_cat
   (hc: (c, s) ~>* (skip, s')):
   (c++c', s) ~>* (skip++c', s') :=
-  RTL.lift (fun (c, s) => (c++c', s)) (fun h => small_step.cat h) hc
+  RTL.lift (fun (c, s) => (c++c', s)) (fun h => cat h) hc
 
 theorem star.cat
   (hc: (c, s) ~>* (skip, s'))
   (hc': (c', s') ~>* (skip, s'')):
   (c++c', s) ~>* (skip, s'') :=
-  RTL.trans (cat_skip_cat hc) (RTL.trans (RTL.single small_step.skipcat) hc')
+  RTL.trans (cat_skip_cat hc) (RTL.trans (RTL.single skipcat) hc')
 
 theorem star.cat_no_influence
   (hc: (c, s) ~>* (skip, s)):
   (c++c', s) ~>* (c', s) :=
-  RTL.trans (cat_skip_cat hc) (RTL.single small_step.skipcat)
+  RTL.trans (cat_skip_cat hc) (RTL.single skipcat)
 
-end Structural
+end SmallStep
 end Com
