Semantics/Imp/Equivalence.lean
@@ -1,42 +1,42 @@
-import Semantics.Imp.Natural
-import Semantics.Imp.Structural
+import Semantics.Imp.BigStep
+import Semantics.Imp.SmallStep
 import Semantics.Imp.Denotational
 
 namespace Com
 
-theorem Structural.from_natural {conf: Com × State}
+theorem SmallStep.from_natural {conf: Com × State}
   (hconf: conf ==> s'): conf ~>* (skip, s') := by
   induction hconf with
   | skip => exact RTL.refl
-  | ass => exact RTL.single small_step.ass
+  | ass => exact RTL.single ass
   | cat _ _ _ ihcatl ihcatr => exact star.cat ihcatl ihcatr
-  | iftrue hcond _ ih => exact RTL.head small_step.ifelse (hcond ▸ ih)
-  | iffalse hcond _ ih => exact RTL.head small_step.ifelse (hcond ▸ ih)
+  | iftrue hcond _ ih => exact RTL.head ifelse (hcond ▸ ih)
+  | iffalse hcond _ ih => exact RTL.head ifelse (hcond ▸ ih)
   | whiletrue _ hcond _ _ ihc ihw =>
-    exact RTL.head small_step.whileloop (RTL.trans (hcond ▸ star.cat ihc ihw) RTL.refl)
+    exact RTL.head whileloop (RTL.trans (hcond ▸ star.cat ihc ihw) RTL.refl)
   | whilefalse hcond =>
-    exact RTL.head small_step.whileloop (hcond ▸ RTL.refl)
+    exact RTL.head whileloop (hcond ▸ RTL.refl)
 
-theorem Natural.from_structural_step
+theorem BigStep.from_structural_step
   (hconf: conf ~> conf') (hconf': conf' ==> s'): conf ==> s' := by
   induction hconf generalizing s' with
-  | ass => exact (skip_eq.mp hconf') ▸ big_step.ass
-  | skipcat => exact big_step.cat _ big_step.skip hconf'
+  | ass => exact (skip_eq.mp hconf') ▸ ass
+  | skipcat => exact cat _ skip hconf'
   | cat _ ih =>
     match hconf' with
-    | big_step.cat s' hcatl hccatr => exact big_step.cat s' (ih hcatl) hccatr
+    | cat s' hcatl hccatr => exact cat s' (ih hcatl) hccatr
   | ifelse => exact if_eq' ▸ hconf'
   | whileloop => rw [loop_unfold]; exact if_eq' ▸ hconf'
 
-theorem Natural.from_structural
-  (hconf: conf ~>* (skip, s')): conf ==> s' := by
+theorem BigStep.from_structural
+  (hconf: conf ~>* (Com.skip, s')): conf ==> s' := by
   induction hconf using RTL.head_induction_on with
-  | refl => exact big_step.skip
+  | refl => exact skip
   | head hsingle _ hs' => exact from_structural_step hsingle hs'
 
 theorem structural_eq_natural:
   ((c, s) ~>* (skip, s')) = ((c, s) ==> s') :=
-  propext (Iff.intro Natural.from_structural Structural.from_natural)
+  propext (Iff.intro BigStep.from_structural SmallStep.from_natural)
 
 theorem denote.from_natural {conf: Com × State}
   (hconf: conf ==> s''): (conf.2, s'') ∈ [[conf.1]] := by
@@ -53,41 +53,41 @@ theorem denote.from_natural {conf: Com × State}
                   and_true]
       exact ih
   | whiletrue s' hcond _ _ ihwhilestep ihwhilerest =>
-    exact while_unfold ▸
+    exact Denotational.while_unfold ▸
       (Or.inl (And.intro
         (Exists.intro s' (And.intro ihwhilestep ihwhilerest)) hcond))
   | whilefalse hcond =>
-      rw [while_unfold]
+      rw [Denotational.while_unfold]
       apply Or.inr
       simp only [Set.mem_diff, Set.mem_comprehend, hcond,
                   Bool.false_eq_true, not_false_eq_true,
                   and_true]
       rfl
 
-theorem Natural.from_denote
+theorem BigStep.from_denote
   (hmem: (s, s'') ∈ [[c]]): (c, s) ==> s'' := by
   revert hmem
   induction c generalizing s s'' with
   | skip =>
     intro hmp
     rw [denote, SFun.mem_id] at hmp
-    exact hmp ▸ big_step.skip
+    exact hmp ▸ skip
   | ass =>
     intro hmp
     rw [denote.eq_def, Set.mem_comprehend] at hmp
     simp only at hmp
-    exact hmp ▸ big_step.ass
+    exact hmp ▸ ass
   | cat _ _ ihcatl ihcatr =>
     intro (Exists.intro s' (And.intro hl hr))
-    exact big_step.cat s' (ihcatl hl) (ihcatr hr)
+    exact cat s' (ihcatl hl) (ihcatr hr)
   | ifelse _ _ _ ih1 ih2 =>
     intro hmp
     match hmp with
     | Or.inl (And.intro hstep hcond) =>
-      exact big_step.iftrue hcond (ih1 hstep)
+      exact iftrue hcond (ih1 hstep)
     | Or.inr (And.intro hstep hcond) =>
       simp only [Set.mem_comprehend, Bool.not_eq_true] at hcond
-      exact big_step.iffalse hcond (ih2 hstep)
+      exact iffalse hcond (ih2 hstep)
   | whileloop b c ih =>
     suffices
       [[while b loop c end]] ⊆ {(s, s'') | (while b loop c end, s) ==> s''} by
@@ -97,14 +97,14 @@ theorem Natural.from_denote
     intro (_, _) hmp
     match hmp with
     | Or.inl (And.intro (Exists.intro s' (And.intro hstep hrest)) hcond) =>
-      exact big_step.whiletrue s' hcond (ih hstep) hrest
+      exact whiletrue s' hcond (ih hstep) hrest
     | Or.inr (And.intro hid hcond) =>
       simp only [Set.mem_comprehend, Bool.not_eq_true] at hcond
       rw [SFun.mem_id] at hid
-      exact hid ▸ big_step.whilefalse hcond
+      exact hid ▸ whilefalse hcond
 
 theorem natural_eq_denote: ((s, s') ∈ [[c]]) = ((c, s) ==> s') :=
-  propext (Iff.intro Natural.from_denote denote.from_natural)
+  propext (Iff.intro BigStep.from_denote denote.from_natural)
 
 theorem structural_eq_denote:
   ((c, s) ~>* (skip, s')) = ((s, s') ∈ [[c]]) :=
